theories/Compositional_Structures/Elect_Composition_Ref.thy
@@ -33,32 +33,6 @@ lemma elector_opt_eq:
   by (simp add: case_prod_beta')
   
 
-(*lemma elector_opt_correct_nres: 
-  fixes m_opt :: "('a set \<Rightarrow> 'a Profile \<Rightarrow> 'a Result nres)"
-fixes m :: "'a Electoral_Module"
-assumes em_m: "electoral_module m" 
-assumes mref: "(uncurry m_opt, uncurry (RETURN oo m)) \<in>  
-  [\<lambda> (A, p). finite_profile A p]\<^sub>f (\<langle>Id\<rangle>set_rel \<times>\<^sub>r \<langle>\<langle>Id \<times>\<^sub>r Id\<rangle>set_rel\<rangle>list_rel) \<rightarrow> 
-   \<langle>\<langle>Id\<rangle>set_rel \<times>\<^sub>r \<langle>Id\<rangle>set_rel \<times>\<^sub>r \<langle>Id\<rangle>set_rel\<rangle>nres_rel"
-shows "(uncurry (elector_opt (m)), uncurry ((elector m))) \<in>
-  [\<lambda> (A, p). finite_profile A p]\<^sub>f (\<langle>Id\<rangle>set_rel \<times>\<^sub>r \<langle>\<langle>Id \<times>\<^sub>r Id\<rangle>set_rel\<rangle>list_rel) \<rightarrow> 
-  \<langle>\<langle>Id\<rangle>set_rel \<times>\<^sub>r \<langle>Id\<rangle>set_rel \<times>\<^sub>r \<langle>Id\<rangle>set_rel\<rangle>nres_rel"
-  unfolding elector_opt_def
-  apply (intro frefI nres_relI) apply clarsimp
-proof (rename_tac A p, refine_vcg, unfold SPEC_eq_is_RETURN)
-  fix A :: "'a set"
-  fix p :: "'a Profile"
-  assume fina: "finite A"
-  assume prof: "profile A p"
-  have mret: "m_opt A p \<le> RETURN (m A p)"
-     using mref[THEN frefD, THEN nres_relD] fina prof
-     by clarsimp
-  thus " m_opt A p
-           \<le> SPEC (\<lambda>x. (case x of (e, r, d) \<Rightarrow> RETURN (e \<union> d, r, {}))
-                        \<le> RETURN (elect m A p \<union> defer m A p, reject m A p, {}))"
-    by (simp add: case_prod_beta' order_trans)
-qed*)
-
 locale Elector_Impl =
   fixes m :: "'a::{default, heap, hashable} Electoral_Module"
   fixes m_sep :: "'a::{default, heap, hashable} Electoral_Module_Sep"
